\section{Continuity}

\subsection{Definitions}

A function $f$ is \textbf{continuous} at $a$ when
\[\lim_{x\to a}f(x)=f(a)\]

Inlining $\epsilon-\delta$ definition, $f$ is continuous at $a$ if for all $\epsilon>0$ there exists $\delta>0$ such that $|x-a|<\delta$ implies $|f(x)-f(a)|<\delta$. Note:
\begin{itemize}
    \item $|f(x)-f(a)|<\delta$ simply says $f(a)$ is the limit.
    \item we drop "$0<$" from $|x-a|<\delta$ because when $x=a$ in continuous functions, $f(x)-f(a)=0$ and thus we're free to examine the value of $f(a)$.
\end{itemize}

A function $f$ is \textbf{continuous on an interval} $(a, b)$ if it's continuous at all $c\in(a,b)$\footnote{Closed intervals are a tiny bit harder, and I'm keeping them out for brevity.}.

\subsection{Building blocks}
The following theorems allow us to tell at a glance that large classes of functions are continuous (e.g. polynomials, rational functions, etc.)

\subsubsection{Easy proofs}
\textbf{Constants}. Let $f(x)=c$. Then $f$ is continuous at all $a$ because $\lim_{x\to a}f(x)=c=f(a)$.

\vs

\textbf{Identity}. Let $f(x)=x$. Then $f$ is continuous at all $a$ because $\lim_{x\to a}f(x)=a=f(a)$.

\vs

\textbf{Addition}. Let $f,g\in\R\to\R$ be continuous at $a$. Then $f+g$ is continuous at $a$ because
\[\lim_{x\to a}(f+g)(x)=\lim_{x\to a}f(x)+\lim_{x\to a}g(x)=f(a)+g(a)=(f+g)(a)\]

\textbf{Multiplication}. Let $f,g\in\R\to\R$ be continuous at $a$. Then $f\cdot g$ is continuous at $a$ because
\[\lim_{x\to a}(fg)(x)=\lim_{x\to a}f(x)\cdot\lim_{x\to a}g(x)=f(a)g(a)=(fg)(a)\]

\textbf{Reciprocal}. Let $f$ be continuous at $a$. Then $\frac{1}{g}$ is continuous at $a$ where $g(a)\neq 0$ because
\[\lim_{x\to a}\left(\frac{1}{g}\right)(x)=\frac{1}{\lim_{x\to a}g(x)}=\frac{1}{g(a)}=\left(\frac{1}{g}\right)(a)\]
(recall that we proved in the limits chapter that $\frac{1}{g}$ is defined.)

\subsubsection{Composition}
Let $f,g\in\R\to\R$. Let $g$ be continuous at $a$, and let $f$ be continuous at $g(a)$. Then $f\circ g$ is continuous at $a$. Put differently, we want to show
\[\lim_{x\to a}(f\circ g)(x)=(f\circ g)(a)\]

Unpacking the definitions, let $\epsilon>0$ be given. We want to show there exists $\delta>0$ such that $|x-a|<\delta$ implies
\begin{align*}
    |(f\circ g)&(x)-(f\circ g)(a)|\\
    &=|f(g(x))-f(g(a))|<\epsilon
\end{align*}

By problem statement we have two continuities.

\vs

\textbf{First}, $f$ is continuous at $g(a)$, i.e. $\lim_{y\to g(a)}f(y)=f(g(a))$. Thus there exists $\delta'>0$ such that $|y-g(a)|<\delta'$ implies $|f(y)-f(g(a))|<\epsilon$.

\vs

\textbf{Second}, $g$ is continuous at $a$, i.e. $\lim_{x\to a}g(x)=g(a)$. Thus there exists $\delta>0$ such that $|x-a|<\delta$ implies $|g(x)-g(a)|<\epsilon$. Since we can make $\epsilon$ be anything, we can set it to $\delta'$.

\vs

I.e. there exists $\delta>0$ such that $|x-a|<\delta$ implies $|g(x)-g(a)|<\delta'$. Which by the first statement implies $|f(g(x))-f(g(a))|<\epsilon$, as desired.

\subsection{Appendix: fun examples}

%%% Local Variables:
%%% TeX-master: "notes"
%%% End:
